core/effect_interpolation_try.v
@@ -21,56 +21,56 @@ Require Import pure.
 Require Import full_composition.
 
 
-Lemma EFF_interp_II_strong: forall m1 m2 nu12 
-                                   (MInj12 : Mem.inject (as_inj nu12) m1 m2) m1'
-                                   (Fwd1: mem_forward m1 m1') nu23 m3
-                                   (MInj23 : Mem.inject (as_inj nu23) m2 m3) m3'
-                                   (Fwd3: mem_forward m3 m3')
-                                   nu' (WDnu' : SM_wd nu')
-                                   (SMvalNu' : sm_valid nu' m1' m3')
-                                   (MemInjNu' : Mem.inject (as_inj nu') m1' m3')
-                                   
-                                   (ExtIncr: extern_incr (compose_sm nu12 nu23) nu')
-                                   (SMV12: sm_valid nu12 m1 m2)
-                                   (SMV23: sm_valid nu23 m2 m3)
-                                   (UnchPrivSrc: Mem.unchanged_on (fun b ofs => locBlocksSrc (compose_sm nu12 nu23) b = true /\ 
-                                                                                pubBlocksSrc (compose_sm nu12 nu23) b = false) m1 m1') 
-                                   (UnchLOOR13: Mem.unchanged_on (local_out_of_reach (compose_sm nu12 nu23) m1) m3 m3')
-
-                                   (GlueInvNu: SM_wd nu12 /\ SM_wd nu23 /\
-                                               locBlocksTgt nu12 = locBlocksSrc nu23 /\
-                                               extBlocksTgt nu12 = extBlocksSrc nu23 /\
-                                               (forall b, pubBlocksTgt nu12 b = true -> 
-                                                          pubBlocksSrc nu23 b = true) /\
-                                               (forall b, frgnBlocksTgt nu12 b = true -> 
-                                                          frgnBlocksSrc nu23 b = true))
-                                   (Norm12: forall b1 b2 d1, extern_of nu12 b1 = Some(b2,d1) ->
-                                                             exists b3 d2, extern_of nu23 b2 = Some(b3, d2))
-                                   (full: full_ext nu12 nu23),
-                            exists m2', exists nu12', exists nu23', nu'=compose_sm nu12' nu23' /\
-                                                                    extern_incr nu12 nu12' /\ extern_incr nu23 nu23' /\
-                                                                    Mem.inject (as_inj nu12') m1' m2' /\ mem_forward m2 m2' /\
-                                                                    Mem.inject (as_inj nu23') m2' m3' /\
-                                                                    sm_valid nu12' m1' m2' /\ sm_valid nu23' m2' m3' /\
-                                                                    (SM_wd nu12' /\ SM_wd nu23' /\
-                                                                     locBlocksTgt nu12' = locBlocksSrc nu23' /\
-                                                                     extBlocksTgt nu12' = extBlocksSrc nu23' /\
-                                                                     (forall b, pubBlocksTgt nu12' b = true -> 
-                                                                                pubBlocksSrc nu23' b = true) /\
-                                                                     (forall b, frgnBlocksTgt nu12' b = true -> 
-                                                                                frgnBlocksSrc nu23' b = true)) /\
-                                                                    (forall b1 b2 d1, extern_of nu12' b1 = Some(b2,d1) ->
-                                                                                      exists b3 d2, extern_of nu23' b2 = Some(b3, d2)) /\ 
-                                                                    Mem.unchanged_on (fun b ofs => locBlocksSrc nu23 b = true /\ 
-                                                                                                   pubBlocksSrc nu23 b = false) m2 m2' /\
-                                                                    Mem.unchanged_on (local_out_of_reach nu12 m1) m2 m2' /\
-                                                                    (*             Mem.unchanged_on (local_out_of_reach nu23 m2) m3 m3' /\*)
-                                                                    (forall b1 b2 d1, as_inj nu12' b1 = Some(b2,d1) -> 
-                                                                                      as_inj nu12 b1 = Some(b2,d1) \/
-                                                                                      exists b3 d, as_inj nu' b1 = Some(b3,d)) /\
-                                                                    (forall b2 b3 d2, as_inj nu23' b2 = Some(b3,d2) -> 
-                                                                                      as_inj nu23 b2 = Some(b3,d2) \/
-                                                                                      exists b1 d, as_inj nu' b1 = Some(b3,d)).
+Lemma EFF_interp_II_strong: 
+  forall m1 m2 nu12 
+         (MInj12 : Mem.inject (as_inj nu12) m1 m2) m1'
+         (Fwd1: mem_forward m1 m1') nu23 m3
+         (MInj23 : Mem.inject (as_inj nu23) m2 m3) m3'
+         (Fwd3: mem_forward m3 m3')
+         nu' (WDnu' : SM_wd nu')
+         (SMvalNu' : sm_valid nu' m1' m3')
+         (MemInjNu' : Mem.inject (as_inj nu') m1' m3')
+         (ExtIncr: extern_incr (compose_sm nu12 nu23) nu')
+         (SMV12: sm_valid nu12 m1 m2)
+         (SMV23: sm_valid nu23 m2 m3)
+         (UnchPrivSrc: Mem.unchanged_on 
+                         (fun b ofs => locBlocksSrc (compose_sm nu12 nu23) b = true /\ 
+                                       pubBlocksSrc (compose_sm nu12 nu23) b = false) m1 m1') 
+         (UnchLOOR13: Mem.unchanged_on (local_out_of_reach (compose_sm nu12 nu23) m1) m3 m3')
+         (GlueInvNu: SM_wd nu12 /\ SM_wd nu23 /\
+                     locBlocksTgt nu12 = locBlocksSrc nu23 /\
+                     extBlocksTgt nu12 = extBlocksSrc nu23 /\
+                     (forall b, pubBlocksTgt nu12 b = true -> 
+                                pubBlocksSrc nu23 b = true) /\
+                     (forall b, frgnBlocksTgt nu12 b = true -> 
+                                frgnBlocksSrc nu23 b = true))
+         (Norm12: forall b1 b2 d1, extern_of nu12 b1 = Some(b2,d1) ->
+                                   exists b3 d2, extern_of nu23 b2 = Some(b3, d2))
+         (full: full_ext nu12 nu23),
+  exists m2', exists nu12', exists nu23', nu'=compose_sm nu12' nu23' /\
+                                          extern_incr nu12 nu12' /\ extern_incr nu23 nu23' /\
+                                          Mem.inject (as_inj nu12') m1' m2' /\ mem_forward m2 m2' /\
+                                          Mem.inject (as_inj nu23') m2' m3' /\
+                                          sm_valid nu12' m1' m2' /\ sm_valid nu23' m2' m3' /\
+                                          (SM_wd nu12' /\ SM_wd nu23' /\
+                                           locBlocksTgt nu12' = locBlocksSrc nu23' /\
+                                           extBlocksTgt nu12' = extBlocksSrc nu23' /\
+                                           (forall b, pubBlocksTgt nu12' b = true -> 
+                                                      pubBlocksSrc nu23' b = true) /\
+                                           (forall b, frgnBlocksTgt nu12' b = true -> 
+                                                      frgnBlocksSrc nu23' b = true)) /\
+                                          (forall b1 b2 d1, extern_of nu12' b1 = Some(b2,d1) ->
+                                                            exists b3 d2, extern_of nu23' b2 = Some(b3, d2)) /\ 
+                                          Mem.unchanged_on (fun b ofs => locBlocksSrc nu23 b = true /\ 
+                                                                         pubBlocksSrc nu23 b = false) m2 m2' /\
+                                          Mem.unchanged_on (local_out_of_reach nu12 m1) m2 m2' /\
+                                          (*             Mem.unchanged_on (local_out_of_reach nu23 m2) m3 m3' /\*)
+                                          (forall b1 b2 d1, as_inj nu12' b1 = Some(b2,d1) -> 
+                                                            as_inj nu12 b1 = Some(b2,d1) \/
+                                                            exists b3 d, as_inj nu' b1 = Some(b3,d)) /\
+                                          (forall b2 b3 d2, as_inj nu23' b2 = Some(b3,d2) -> 
+                                                            as_inj nu23 b2 = Some(b3,d2) \/
+                                                            exists b1 d, as_inj nu' b1 = Some(b3,d)).
 (*                   (forall b1 b2 ofs2, as_inj nu12' b1 = Some(b2,ofs2) -> 
                      (as_inj nu12 b1 = Some (b2,ofs2)) \/
                      (b1 = Mem.nextblock m1 /\ b2 = Mem.nextblock m2 /\ ofs2 = 0) \/ 
@@ -90,10 +90,11 @@ Proof. intros.
          remember (bconcat (extBlocksSrc nu23) (extBlocksSrc nu') sizeM2) as extS23;
          remember (extBlocksTgt nu') as extT23;
          remember (mkInjections (Mem.nextblock m2) j k l') as output;
+         remember (join (j) (restrict (local_of nu12) (pubBlocksSrc nu12))) as jp;
          destruct output as [j' k'].
        remember (change_ext nu12 extS12 extT12 j') as nu12';
          remember (change_ext nu23 extS23 extT23 k') as nu23'.
-       exists (mem_add m2 m1'), nu12', nu23'.
+       exists (mem_add jp m2 m1'), nu12', nu23'.
        split.
        
        (*Compose_sm*)
@@ -134,26 +135,375 @@ Proof. intros.
        }
        split.
        (* Mem.inject *)
-       { destruct MInj12. constructor.
-         + destruct mi_inj. constructor.
-           - move mi_perm at bottom.
-             intros. unfold Mem.perm. rewrite mem_add_accx; unfold mem_add_acc.
-             subst nu12'. unfold change_ext, as_inj, join in H. destruct nu12; simpl in H.
-             inversion Heqoutput; subst j'. unfold add_inj, shiftT in H.
-              destruct (j b1) eqn:jb1. destruct p0. inversion H.
-              subst j. unfold as_inj, join in mi_perm; simpl in *. 
-              apply mi_perm.
-              rewrite jb1 in mi_perm.
-              apply SMV12.
+       { constructor.
+         + constructor.
+         - { intros b1 b2 delta ofs k0 per H H0.
+             unfold Mem.perm; rewrite (mem_add_accx jp m1' m2); unfold mem_add_acc.
+             (* New trying things*)
+             unfold as_inj in H; apply joinD_Some in H; destruct H as [extmap | [extNone locmap]].
+             + subst nu12'; rewrite ext_change_ext in extmap.
+               eapply MKI_Some12 in extmap; eauto. 
+               destruct extmap as [jmap | [jmap [b2' [d' [lmap' [b2eq deltaeq]]]]]].
+             - assert (Mem.valid_block m2 b2).
+               { apply SMV12. unfold RNG, DomTgt. subst j; apply GlueInvNu in jmap. 
+                 destruct jmap as [extS extT]; rewrite extT; apply orb_true_r. }
+               destruct (valid_dec m2 b2); try solve[contradict n; auto].
+               erewrite source_SomeI. apply H0.
+               * eapply meminj_no_overlap_inject_incr.
+                 eapply (no_overlap_forward _ _ _ _ SMV12); eauto.
+                 apply GlueInvNu.
+                 apply MInj12.
+                 subst jp. apply inject_incr_join.
+                 subst j; apply inject_incr_refl.
+                 eapply inject_incr_trans; [eapply restrict_incr | apply inject_incr_refl].
+                 apply disjoint_extern_local; eauto.
+                 apply GlueInvNu.
+               *  subst jp; unfold join; rewrite jmap; auto.
+               * eapply any_Max_Nonempty; eauto.
+             - destruct (valid_dec m2 b2); (*first discharge the impossible case*)
+               try solve[subst b2; contradict v; unfold Mem.valid_block; xomega].
+               subst b2 delta. rewrite Pos.add_sub; auto.
+               replace (ofs + 0) with ofs by omega; trivial.
+             + subst nu12'; rewrite loc_change_ext in locmap.
+               rewrite ext_change_ext in extNone.
+               assert (Mem.valid_block m2 b2).
+               { apply SMV12. unfold RNG, DomTgt. apply GlueInvNu in locmap. 
+                 destruct locmap as [locS locT]; rewrite locT; apply orb_true_l. }
+               destruct (valid_dec m2 b2); try solve[contradict n; auto].
+               destruct (source jp m1' b2 (ofs + delta)) eqn:sour.
+               - destruct p; symmetry in sour.
+                 destruct (source_SomeE _ _ _ _ _ sour) 
+                               as [b1' [delta' [ofs1 [pairs [bval [jpmap [mperm ofss]]]]]]].
+                 inversion pairs; subst b z jp.
+                 (*b2 is local so j can't map to it *)
+                 unfold join in jpmap.
+                 destruct (j b1') eqn:jmap; try destruct p.
+                 {inversion jpmap; subst b z j.
+                 apply GlueInvNu in jmap; destruct jmap as [extS extT].
+                 apply GlueInvNu in locmap; destruct locmap as [locS locT].
+                 destruct GlueInvNu as [SMWD12 rest]; clear rest.
+                 destruct SMWD12. destruct (disjoint_extern_local_Tgt b2) as [LT | ET];
+                 [rewrite LT in locT | rewrite ET in extT]; discriminate. }
+                 apply restrictD_Some in jpmap; destruct jpmap as [locmap' pubtrue].
+                 Lemma no_overlap_no_doublemap: 
+                   forall j b1 b1' b2 d d' m,
+                     Mem.meminj_no_overlap j m ->
+                     j b1 = Some (b2, d) ->
+                     j b1' = Some (b2, d') ->
+                     forall ofs ofs',
+                       Mem.perm m b1 ofs Max Nonempty ->
+                       Mem.perm m b1' ofs' Max Nonempty ->
+                       ofs + d = ofs' + d' ->
+                       b1' = b1 /\ ofs = ofs' /\ d = d'.
+                   intros.
+                   destruct (peq b1 b1'). 
+                   { subst b1. rewrite H1 in H0; inversion H0. 
+                     subst d'; assert (ofs = ofs') by xomega. intuition. }
+                   destruct (H b1 b2 d b1' b2 d' ofs ofs') as [H5 | H5]; eauto;
+                   contradiction H5; auto.
+                 Qed.
+                 edestruct (no_overlap_no_doublemap (local_of nu12) b1 b1') as 
+                     [b1_eq [ofs_eq d_eq]]; eauto.
+                 { eapply meminj_no_overlap_inject_incr.
+                   eapply no_overlap_forward. 
+                   apply SMV12.
+                   apply GlueInvNu.
+                   auto.
+                   apply MInj12.
+                   apply local_in_all. apply GlueInvNu. }
+                 eapply any_Max_Nonempty; eauto.
+                 subst b1' ofs1; auto.
+               - destruct MInj12.
+                 destruct mi_inj.
+                 eapply mi_perm0.
+                 apply local_in_all; eauto.
+                 apply GlueInvNu. 
+                 apply UnchPrivSrc.
+                 unfold compose_sm; simpl.
+                 assert (locmap':=locmap).
+                 apply GlueInvNu in locmap'; destruct locmap' as [locS locT].
+                 rewrite locS; simpl; split; auto.
+                 destruct (pubBlocksSrc nu12 b1) eqn:pubTrue; trivial.
+                 assert (pubS:=pubTrue).
+                 apply GlueInvNu in pubTrue. destruct pubTrue as [b2' [z [locmap' pubT]]].
+                 rewrite locmap in locmap'; inversion locmap'; subst b2 delta. clear locmap'.
+                 assert (jp b1 = Some (b2', z)).
+                 { subst jp. unfold join. 
+                   rewrite (inject_incr_inv j j'); eauto.
+                   unfold restrict. rewrite pubS.
+                   auto.
+                   eapply MKI_incr12; eauto. }
+                 symmetry in sour.
+                 eapply any_Max_Nonempty in H0.
+                 contradict H0.
+                 replace ofs with ((ofs + z) - z) by omega.
+                 eapply source_NoneE; eauto.
+                 (*The three remaining goals follow the same logic*)
+                 assert (Mem.valid_block m1 b1).
+                 { destruct SMV12 as [Dv Rv]; clear Rv.
+                   apply Dv. unfold DOM, DomSrc.
+                   rewrite locS; auto.
+                 }
+                 apply Fwd1 in H0; destruct H0 as [H0 ?].
+                 apply H0.
 
-             destruct (j' b1) eqn:jb1.
-             * destruct p0. inversion H; inversion Heqoutput. subst b j'.
-               unfold add_inj, shiftT in jb1.
-             
- admit. }
+                 destruct SMV12 as [Dv Rv]; clear Rv.
+                 apply Dv. unfold DOM, DomSrc.
+                 apply GlueInvNu in locmap; destruct locmap as [locS locT].
+                 rewrite locS; auto.
+                 
+                 auto.
+               }
+         - intros. unfold Z.divide.
+           subst nu12'; unfold as_inj, join in H. rewrite ext_change_ext, loc_change_ext in H.
+           destruct (j' b1) eqn:jmap'. 
+           destruct p0. destruct (MKI_Some12 _ _ _ _ _ _ Heqoutput _ _ _ jmap') as 
+                          [jmap | [jmap [b2' [d' [lmap [b2eq deq]]]]]].
+           inversion H; subst b z.
+           subst j. destruct MInj12. destruct mi_inj.
+           eapply (mi_align b1 b2); eauto. 
+           unfold as_inj, join; rewrite jmap; trivial.
+           Lemma forward_range:
+             forall m m' b ofs size p,
+               mem_forward m m' ->
+               Mem.valid_block m b ->
+               Mem.range_perm m' b ofs (ofs + size) Max p ->
+               Mem.range_perm m b ofs (ofs + size) Max p.
+             unfold Mem.range_perm; intros.
+             apply H; auto.
+           Qed.
+           eapply forward_range; eauto.
+           clear H. 
+           Lemma mapped_valid: forall mu m1 m2 b1 b2 d,
+                                 SM_wd mu ->
+                                 as_inj mu b1 = Some (b2, d) ->
+                                 sm_valid mu m1 m2 ->
+                                 Mem.valid_block m1 b1.
+             intros. destruct H1 as [H1 H2]; apply H1.
+             unfold DOM, DomSrc.
+             apply joinD_Some in H0; destruct H0 as [map | [extNone map]];
+             apply H in map; destruct map as [src tgt]; rewrite src; auto.
+             apply orb_true_r.
+           Qed.
+           eapply mapped_valid.
+           destruct GlueInvNu as [SMWD12 rest]; apply SMWD12. 
+           unfold as_inj, join; rewrite jmap; auto. 
+           eauto.
+           
+           (* This should be folded in a lemma *)
+           inversion Heqoutput.
+           unfold add_inj, shiftT in H2. subst j'. rewrite jmap in jmap'.
+           unfold filter_id in jmap'. rewrite lmap in jmap'.
+           inversion jmap'. subst z. symmetry in H; inversion H; subst delta.
+           exists 0; xomega.
+           (*Done *)
+           
+           destruct MInj12. destruct mi_inj.
+           eapply (mi_align b1 b2); eauto.
+           unfold as_inj. 
+           rewrite join_com. 
+           unfold join; rewrite H; trivial.
+           apply disjoint_extern_local.
+           apply GlueInvNu.
+           eapply forward_range; eauto.
+           eapply mapped_valid.
+           destruct GlueInvNu as [SMWD12 rest]; apply SMWD12. 
+           unfold as_inj. 
+           rewrite join_com. 
+           unfold join; rewrite H; trivial.
+           apply disjoint_extern_local.
+           apply GlueInvNu.
+           eauto.
+         - intros. rewrite mem_add_contx.          
+           subst nu12'. unfold as_inj in H. rewrite ext_change_ext, loc_change_ext in H.
+           apply joinD_Some in H; destruct H as [ jmap' | [jmap' locmap] ].
+           apply (MKI_Some12 _ _ _ _ _ _ Heqoutput) in jmap'.
+           destruct jmap' as [jmap | [jmap [b2' [d' [lmap [b2eq deq]]]]]].
+           destruct MInj12; destruct mi_inj. 
+           assert (b1val: Mem.valid_block m1 b1).
+           { eapply mapped_valid. destruct GlueInvNu as [SMWD12 rest]; apply SMWD12.
+             subst j; unfold as_inj, join; rewrite jmap. reflexivity.
+             eauto. }
+           apply Fwd1 in b1val. destruct b1val as [b1val' mpermm].
+           apply mpermm in H0.
+           inversion (mi_memval b1 ofs b2 delta).
+           constructor.
+           apply mi_memval.
+
+
+       + intros. unfold as_inj; subst nu12'; rewrite ext_change_ext, loc_change_ext.
+         assert (H0: ~ Mem.valid_block m1 b). 
+         { clear - H Fwd1. unfold not, Mem.valid_block in *.
+           intros; apply H. apply (Pos.lt_le_trans _ _ _ H0).
+           apply forward_nextblock; assumption. }
+         destruct MInj12, MemInjNu'.
+         apply mi_freeblocks in H0; destruct (as_injD_None _ _ H0) as [ext loc].
+         apply mi_freeblocks0 in H; destruct (as_injD_None _ _ H) as [ext' loc'].
+         unfold join.
+         erewrite MKI_None12; subst; eauto; subst.
+       + unfold as_inj; subst nu12'.
+         intros b b' delta map; destruct (as_in_SomeE _ _ _ _ map) as [ext | loc].
+         rewrite ext_change_ext in ext. 
+         destruct (MKI_Some12 _ _ _ _ _ _ Heqoutput _ _ _ ext).
+         destruct MInj12.
+         unfold Mem.valid_block; rewrite mem_add_nbx; unfold mem_add_nb.
+         eapply Pos.lt_trans; try eapply (Pos.lt_add_diag_r (Mem.nextblock m2)).
+         apply (mi_mappedblocks b b' delta).
+         unfold as_inj, join; subst; rewrite H; auto.
+         destruct H as [jmap [b2' [d' [lmap' [eq1 eq2]]]]].
+         destruct MemInjNu'. unfold Mem.valid_block; rewrite mem_add_nbx.
+         unfold mem_add_nb. subst b'.
+         destruct WDnu'.
+         subst l'.
+         apply extern_DomRng in lmap'; destruct lmap' as [extS extT].
+         destruct SMvalNu' as [DOMv RNGv].
+         assert (Plt b m1'.(Mem.nextblock)).
+         apply DOMv. unfold DOM, DomSrc. rewrite extS; apply orb_true_r.
+         xomega.
+
+         unfold Mem.valid_block; rewrite mem_add_nbx.
+         unfold mem_add_nb.
+         rewrite loc_change_ext in loc.
+         destruct GlueInvNu as [WDnu12 rest];clear rest; destruct WDnu12.
+         apply local_DomRng in loc; destruct loc as [locS locT].
+         destruct SMV12 as [DOMv RNGv].
+         assert (Plt b' m2.(Mem.nextblock)).
+         apply RNGv. unfold RNG, DomTgt. rewrite locT; apply orb_true_l.
+         xomega.
+       + idtac.
+         Lemma no_overlap_asinj: 
+           forall mu m, 
+             SM_wd mu -> 
+             Mem.meminj_no_overlap (extern_of mu) m ->
+             Mem.meminj_no_overlap (local_of mu) m ->
+             Mem.meminj_no_overlap (as_inj mu) m.
+           unfold Mem.meminj_no_overlap.
+           intros mu m SMWD NOO_ext NOO_loc.
+           intros.
+           apply as_in_SomeE in H0.
+           apply as_in_SomeE in H1.
+           destruct H0 as [ext1 | loc1];
+           destruct H1 as [ext2 | loc2].
+           eapply NOO_ext; eauto.
+           destruct SMWD. apply extern_DomRng in ext1; apply local_DomRng in loc2.
+           destruct (peq b1' b2'); auto; subst b1'.
+           destruct loc2; destruct ext1.
+           destruct (disjoint_extern_local_Tgt b2'). 
+           rewrite H6 in H1; inversion H1.
+           rewrite H6 in H5; inversion H5.
+           destruct SMWD. apply extern_DomRng in ext2; apply local_DomRng in loc1.
+           destruct (peq b1' b2'); auto; subst b1'.
+           destruct loc1; destruct ext2.
+           destruct (disjoint_extern_local_Tgt b2'). 
+           rewrite H6 in H1; inversion H1.
+           rewrite H6 in H5; inversion H5.
+           eapply NOO_loc; eauto.
+         Qed.
+         Lemma no_overlap_ext:
+           forall mu m,
+             Mem.meminj_no_overlap (as_inj mu) m ->
+             Mem.meminj_no_overlap (extern_of mu) m.
+           unfold Mem.meminj_no_overlap; intros.
+           eapply H; eauto.
+           unfold as_inj, join; rewrite H1; auto.
+           unfold as_inj, join; rewrite H2; auto.
+         Qed.
+         Lemma no_overlap_loc:
+           forall mu m,
+             SM_wd mu ->
+             Mem.meminj_no_overlap (as_inj mu) m ->
+             Mem.meminj_no_overlap (local_of mu) m.
+           unfold Mem.meminj_no_overlap; intros.
+           eapply H0; eauto.
+           unfold as_inj; rewrite (join_com _ _ (disjoint_extern_local _ H)); unfold join.
+           rewrite H2; auto.
+           unfold as_inj; rewrite (join_com _ _ (disjoint_extern_local _ H)); unfold join.
+           rewrite H3; auto.
+         Qed.
+         apply no_overlap_asinj.
+         admit.
+         subst nu12'; rewrite ext_change_ext.
+         admit. (* from construction*)
+         subst nu12'; rewrite loc_change_ext.
+         admit.
+       + intros.
+         subst nu12'. apply as_in_SomeE in H; destruct H as [ext1 | loc1];
+         [ rewrite ext_change_ext in ext1 | rewrite loc_change_ext in loc1].
+         - eapply MKI_Some12 in ext1; eauto. 
+           destruct ext1 as [jmap | [jmap [b3 [d [lmap' [beq deq]]]]]].
+           assert (map12: as_inj nu12 b = Some (b', delta)).
+           { unfold as_inj, join ; subst j; rewrite jmap; eauto. }
+           destruct MInj12. eapply mi_representable; eauto. 
+           destruct H0; [left | right].
+           eapply Fwd1.
+           Lemma valid_from_map: 
+             forall mu m1 m2 b1 b2 d,
+               SM_wd mu -> 
+               as_inj mu b1 = Some (b2,d) ->
+               sm_valid mu m1 m2 ->
+               Mem.valid_block m1 b1.
+             intros mu m1 m2 b1 b2 d SMWD map smv. 
+             apply as_in_SomeE in map.
+             destruct SMWD, smv as [DOMv RNGv], map as [ext1 | loc1];
+             apply DOMv; unfold DOM, DomSrc.
+             apply extern_DomRng in ext1; destruct ext1 as [extS extT].
+             rewrite extS; apply orb_true_r.
+             apply local_DomRng in loc1; destruct loc1 as [locS locT].
+             rewrite locS; apply orb_true_l.
+             Qed.
+           eapply valid_from_map. 
+           destruct GlueInvNu as [SMWD12 rest]; apply SMWD12.
+           apply map12.
+           eassumption.
+           assumption.
+
+           eapply Fwd1.
+           eapply valid_from_map. 
+           destruct GlueInvNu as [SMWD12 rest]; apply SMWD12.
+           apply map12.
+           eassumption.
+           assumption.
+
+           destruct ofs as [ofs range].
+           subst delta; split; simpl. 
+           xomega. 
+           split.
+           xomega.
+           unfold Int.max_unsigned.
+           xomega.
+         - assert (map12: as_inj nu12 b = Some (b', delta)).
+           { unfold as_inj. rewrite join_com. unfold join; rewrite loc1; auto.
+             apply disjoint_extern_local; apply GlueInvNu. }
+           destruct MInj12. eapply mi_representable; eauto. 
+           destruct H0; [left | right].
+           eapply Fwd1; eauto.
+           eapply (valid_from_map nu12); eauto.
+           destruct GlueInvNu as [SMWD12 rest]; apply SMWD12.
+           eapply Fwd1; eauto.
+           eapply (valid_from_map nu12); eauto.
+           destruct GlueInvNu as [SMWD12 rest]; apply SMWD12.
+           }
        split.
        (* mem_forward *)
-       { apply mem_add_forward. }
+       { apply (mem_add_forward j' m1' m2 jp m1); auto.
+         + destruct SMV12 as [DOMv RNGv].
+           intros; apply DOMv; unfold DOM, DomSrc. 
+           destruct GlueInvNu as [SMWD12 rest]; clear rest.
+           subst j. destruct SMWD12. destruct p; subst jp. 
+           apply joinD_Some in H; destruct H as [ext1 | [jnone resloc]].
+           - apply extern_DomRng in ext1.
+             destruct ext1 as [extS extT]; rewrite extS; apply orb_true_r.
+           - apply restrictD_Some in resloc; destruct resloc as [loc1 pucTrue].
+             apply local_DomRng in loc1; destruct loc1 as [locS locT]; rewrite locS; auto.
+         (*+ apply (MKI_range_eq _ _ _ _ _ _ Heqoutput).*)
+         + unfold mi_perm; destruct MInj12; destruct mi_inj; auto. 
+           intros; eapply mi_perm0; eauto. 
+           subst j jp; unfold as_inj, join. 
+           apply joinD_Some in H; destruct H as [ext1 | [ext1 loc1]].
+           - rewrite ext1; auto.
+           - apply restrictD_Some in loc1; destruct loc1 as [loc1 pubTrue].
+             rewrite ext1; rewrite loc1; auto.
+       }
        split.
        (* Mem.inject *)
        { admit. }
@@ -379,17 +729,84 @@ Proof. intros.
        }
        split.
        (* Mem.unchanged_on *)
-       { apply (mem_unchanged_on_sub _ _ _ _ (mem_add_unchanged m1' m2)).
-         intros. destruct SMV23 as [DOMval RNGval].
-         apply DOMval. unfold DOM, DomSrc.
-         destruct H. rewrite H; auto.
+       { constructor; intros.
+         + (* If [locBlocksSrc nu23 b] then b has no preimage in j *)
+           assert (no_preimage: source jp m1' b ofs = None).
+           { destruct (source jp m1' b ofs) eqn: preimage; trivial.
+             symmetry in preimage; apply source_SomeE in preimage.
+             destruct preimage as [b1 [delta [ofs1 [po [mvalid [jmap ?]]]]]].
+             subst jp j.
+             apply joinD_Some in jmap; destruct jmap as [jmap | restPub].
+             destruct GlueInvNu as [SMWD12 [SMWD23 [loceq rest]]]; clear SMWD23 rest.
+             apply SMWD12 in jmap; destruct jmap.
+             destruct SMWD12. destruct (disjoint_extern_local_Tgt b).
+             - rewrite loceq in H4.
+               destruct H as [locTrue pubFalse]; rewrite locTrue in H4; inversion H4.
+             - rewrite H3 in H4; inversion H4. 
+               (*This last part follows from the public blocks. Becasue they change.*)
+             - destruct restPub. 
+               unfold restrict in H3. destruct H as [H5 H6].
+               destruct (pubBlocksSrc nu12 b1) eqn:pubS12; try solve[inversion H3].
+               destruct (local_of nu12 b1) eqn:loc12; inversion H3.
+               destruct p1 as [bn dn]; inversion H3.
+               destruct GlueInvNu as [SMWD12 [? [loc [ext [pub frg]]]]].
+               assert (loc12':=loc12).
+               apply SMWD12 in loc12.
+               apply SMWD12 in pubS12. destruct pubS12 as [b2 [z [locmap pubT]]].
+               destruct loc12 as [locS12 locT12].
+               move pub at bottom. 
+               apply pub in pubT.
+               rewrite locmap in loc12'; inversion loc12'.
+               subst bn dn.
+               subst b2.
+               rewrite pubT in H6; inversion H6. 
+           }
+           unfold Mem.perm. 
+           rewrite (mem_add_accx jp m1' m2 b). unfold mem_add_acc.
+           destruct (valid_dec m2 b) as [y | n]; try solve[contradict n; assumption].
+           rewrite no_preimage; split; auto.
+         + admit.
        }
+       (* Mem.unchanged_on *) (*NOTE: hey both Mem.unchanged_on look very alike! *)
        split.
-       { apply (mem_unchanged_on_sub _ _ _ _ (mem_add_unchanged m1' m2)).
-         intros. 
-         destruct SMV12 as [DOMval RNGval].
-         apply RNGval. unfold RNG, DomTgt.
-         destruct H. rewrite H; auto. 
+       { unfold local_out_of_reach.
+         constructor; intros.
+         + destruct H. 
+           unfold Mem.perm.
+           rewrite mem_add_accx; unfold mem_add_acc.
+           destruct (valid_dec m2 b); try contradiction.
+           destruct (source jp m1' b ofs) eqn:sour; try solve[split; trivial].
+           destruct p0; simpl.
+           symmetry in sour; apply source_SomeE in sour.
+           destruct sour as [b1 [d [ofs1 [invertibles[ ineq [jpmap [mperm ofsets]]]]]]].
+           subst jp.
+           (* This will show that local_of nu12 maps b1->b (bc. locBlocksTgt nu12 b = true)*)
+           unfold join in jpmap. destruct (j b1) eqn:jmap.
+           destruct p0; simpl in *.
+           subst j. apply GlueInvNu in jmap; destruct jmap as [extS extT].
+           destruct GlueInvNu as [SMWD12 rest]; clear rest; destruct SMWD12.
+           destruct (disjoint_extern_local_Tgt b2).
+           inversion invertibles; inversion jpmap; subst.
+           rewrite H in H2; inversion H2.
+           rewrite extT in H2; inversion H2.
+           apply restrictD_Some in jpmap; destruct jpmap as [locmap publ].
+           assert (locmap':= locmap).
+           apply H1 in locmap'.
+           destruct locmap' as [notperm | notpub];
+             try solve[rewrite notpub in publ; inversion publ].
+           inversion invertibles; subst b0 z.
+           move Fwd1 at bottom.
+           unfold mem_forward in Fwd1.
+           assert (Mem.valid_block m1 b1).
+           { destruct SMV12 as [DOMv RNGv]; clear RNGv; apply DOMv.
+             unfold DOM, DomSrc. apply GlueInvNu in locmap.
+             destruct locmap as [locS locT]. rewrite locS; auto.
+           }
+           apply Fwd1 in H2; destruct H2 as [bval mperms].
+           apply mperms in mperm. subst ofs. 
+           contradict notperm; replace (ofs1 +d - d) with ofs1 by xomega.
+           assumption.
+         + admit.
        }
        split.
        { intros; subst;
@@ -407,5 +824,59 @@ Proof. intros.
          - right; destruct H0 as [b1 rest]; exists b1, d2; exact rest.
        }
 Qed.
+
+Lemma EFF_interp_II: forall m1 m2 nu12 
+                             (MInj12 : Mem.inject (as_inj nu12) m1 m2) m1'
+                             (Fwd1: mem_forward m1 m1') nu23 m3
+                             (MInj23 : Mem.inject (as_inj nu23) m2 m3) m3'
+                             (Fwd3: mem_forward m3 m3')
+                              nu' (WDnu' : SM_wd nu')
+                             (SMvalNu' : sm_valid nu' m1' m3')
+                             (MemInjNu' : Mem.inject (as_inj nu') m1' m3')
+                             
+                             (ExtIncr: extern_incr (compose_sm nu12 nu23) nu')
+                             (SMInjSep: sm_inject_separated (compose_sm nu12 nu23) nu' m1 m3)
+                             (SMV12: sm_valid nu12 m1 m2)
+                             (SMV23: sm_valid nu23 m2 m3)
+                             (UnchPrivSrc: Mem.unchanged_on (fun b ofs => locBlocksSrc (compose_sm nu12 nu23) b = true /\ 
+                                                      pubBlocksSrc (compose_sm nu12 nu23) b = false) m1 m1') 
+                             (UnchLOOR13: Mem.unchanged_on (local_out_of_reach (compose_sm nu12 nu23) m1) m3 m3')
+
+                             (GlueInvNu: SM_wd nu12 /\ SM_wd nu23 /\
+                                         locBlocksTgt nu12 = locBlocksSrc nu23 /\
+                                         extBlocksTgt nu12 = extBlocksSrc nu23 /\
+                                         (forall b, pubBlocksTgt nu12 b = true -> 
+                                                    pubBlocksSrc nu23 b = true) /\
+                                         (forall b, frgnBlocksTgt nu12 b = true -> 
+                                                    frgnBlocksSrc nu23 b = true))
+                             (Norm12: forall b1 b2 d1, extern_of nu12 b1 = Some(b2,d1) ->
+                                             exists b3 d2, extern_of nu23 b2 = Some(b3, d2))
+                             (full: full_ext nu12 nu23),
+     exists m2', exists nu12', exists nu23', nu'=compose_sm nu12' nu23' /\
+                             extern_incr nu12 nu12' /\ extern_incr nu23 nu23' /\
+                             Mem.inject (as_inj nu12') m1' m2' /\ mem_forward m2 m2' /\
+                             Mem.inject (as_inj nu23') m2' m3' /\
+                             sm_valid nu12' m1' m2' /\ sm_valid nu23' m2' m3' /\
+                             (SM_wd nu12' /\ SM_wd nu23' /\
+                              locBlocksTgt nu12' = locBlocksSrc nu23' /\
+                              extBlocksTgt nu12' = extBlocksSrc nu23' /\
+                              (forall b, pubBlocksTgt nu12' b = true -> 
+                                         pubBlocksSrc nu23' b = true) /\
+                              (forall b, frgnBlocksTgt nu12' b = true -> 
+                                         frgnBlocksSrc nu23' b = true)) /\
+                             (forall b1 b2 d1, extern_of nu12' b1 = Some(b2,d1) ->
+                                     exists b3 d2, extern_of nu23' b2 = Some(b3, d2)) /\ 
+                              Mem.unchanged_on (fun b ofs => locBlocksSrc nu23 b = true /\ 
+                                                             pubBlocksSrc nu23 b = false) m2 m2' /\
+                              Mem.unchanged_on (local_out_of_reach nu12 m1) m2 m2' 
+                          (* /\ Mem.unchanged_on (local_out_of_reach nu23 m2) m3 m3'*).
+Proof. intros.
+  destruct (EFF_interp_II_strong _ _ _ MInj12 _ Fwd1 _ _ MInj23 _ 
+              Fwd3 _ WDnu' SMvalNu' MemInjNu' ExtIncr
+              SMV12 SMV23 UnchPrivSrc UnchLOOR13 GlueInvNu Norm12 full)
+  as [m2' [nu12' [nu23' [A [B [C [D [E [F [G [H [I [J [K [L [M ]]]]]]]]]]]]]]]].
+  exists m2', nu12', nu23'. intuition.
+Qed.
+
 
 
